Start updating the Scalar definition to use bit vectors

backends/lean/Aeneas/Std/ScalarCore.lean
@@ -13,89 +13,110 @@ namespace Std
 -- Deactivate the warnings which appear when we use `#assert`
 set_option linter.hashCommand false
 
-----------------------
--- MACHINE INTEGERS --
-----------------------
+/-!
+# Machine Integers
+
+Because they tend to behave quite differently, we have two classes of machine integers: one for
+signed integers, and another for unsigned integers. Inside of each class, we factor out definitions.
+-/
 
 open Result Error
 open System.Platform.getNumBits
 
 -- TODO: is there a way of only importing System.Platform.getNumBits?
---
-@[simp] def size_num_bits : Nat := (System.Platform.getNumBits ()).val
+@[simp] def size_num_bits : Nat := System.Platform.numBits
 
 -- Remark: Lean seems to use < for the comparisons with the upper bounds by convention.
 
--- The "structured" bounds
-def Isize.smin : Int := - (HPow.hPow 2 (size_num_bits - 1))
-def Isize.smax : Int := (HPow.hPow 2 (size_num_bits - 1)) - 1
-def I8.smin    : Int := - (HPow.hPow 2 7)
-def I8.smax    : Int := HPow.hPow 2 7 - 1
-def I16.smin   : Int := - (HPow.hPow 2 15)
-def I16.smax   : Int := HPow.hPow 2 15 - 1
-def I32.smin   : Int := -(HPow.hPow 2 31)
-def I32.smax   : Int := HPow.hPow 2 31 - 1
-def I64.smin   : Int := -(HPow.hPow 2 63)
-def I64.smax   : Int := HPow.hPow 2 63 - 1
-def I128.smin  : Int := -(HPow.hPow 2 127)
-def I128.smax  : Int := HPow.hPow 2 127 - 1
-def Usize.smin : Nat := 0
-def Usize.smax : Nat := HPow.hPow 2 size_num_bits - 1
-def U8.smin    : Nat := 0
-def U8.smax    : Nat := HPow.hPow 2 8 - 1
-def U16.smin   : Nat := 0
-def U16.smax   : Nat := HPow.hPow 2 16 - 1
-def U32.smin   : Nat := 0
-def U32.smax   : Nat := HPow.hPow 2 32 - 1
-def U64.smin   : Nat := 0
-def U64.smax   : Nat := HPow.hPow 2 64 - 1
-def U128.smin  : Nat := 0
-def U128.smax  : Nat := HPow.hPow 2 128 - 1
+/-- Kinds of unsigned integers -/
+inductive UScalarTy where
+| Usize
+| U8
+| U16
+| U32
+| U64
+| U128
 
--- The "normalized" bounds, that we use in practice
-def I8.min    : Int   := -128
-def I8.max    : Int   := 127
-def I16.min   : Int  := -32768
-def I16.max   : Int  := 32767
-def I32.min   : Int  := -2147483648
-def I32.max   : Int  := 2147483647
-def I64.min   : Int  := -9223372036854775808
-def I64.max   : Int  := 9223372036854775807
-def I128.min  : Int := -170141183460469231731687303715884105728
-def I128.max  : Int := 170141183460469231731687303715884105727
-@[simp]
-def U8.min    : Nat   := 0
-def U8.max    : Nat   := 255
-@[simp]
-def U16.min   : Nat  := 0
-def U16.max   : Nat  := 65535
-@[simp]
-def U32.min   : Nat  := 0
-def U32.max   : Nat  := 4294967295
-@[simp]
-def U64.min   : Nat  := 0
-def U64.max   : Nat  := 18446744073709551615
-@[simp]
-def U128.min  : Nat := 0
-def U128.max  : Nat := 340282366920938463463374607431768211455
-@[simp]
-def Usize.min : Nat := 0
+/-- Kinds of signed integers -/
+inductive IScalarTy where
+| Isize
+| I8
+| I16
+| I32
+| I64
+| I128
+
+def UScalarTy.bitWidth (ty : UScalarTy) : Nat :=
+  match ty with
+  | Usize => size_num_bits
+  | U8 => 8
+  | U16 => 16
+  | U32 => 32
+  | U64 => 64
+  | U128 => 128
+
+def IScalarTy.bitWidth (ty : IScalarTy) : Nat :=
+  match ty with
+  | Isize => size_num_bits
+  | I8 => 8
+  | I16 => 16
+  | I32 => 32
+  | I64 => 64
+  | I128 => 128
+
+@[simp] theorem UScalarTy.Usize_bitWidth_eq : Usize.bitWidth = size_num_bits := by rfl
+@[simp] theorem UScalarTy.U8_bitWidth_eq    : U8.bitWidth    = 8 := by rfl
+@[simp] theorem UScalarTy.U16_bitWidth_eq   : U16.bitWidth   = 16 := by rfl
+@[simp] theorem UScalarTy.U32_bitWidth_eq   : U32.bitWidth   = 32 := by rfl
+@[simp] theorem UScalarTy.U64_bitWidth_eq   : U64.bitWidth   = 64 := by rfl
+@[simp] theorem UScalarTy.U128_bitWidth_eq  : U128.bitWidth  = 128 := by rfl
+
+@[simp] theorem IScalarTy.Isize_bitWidth_eq : Isize.bitWidth = size_num_bits := by rfl
+@[simp] theorem IScalarTy.I8_bitWidth_eq    : I8.bitWidth    = 8 := by rfl
+@[simp] theorem IScalarTy.I16_bitWidth_eq   : I16.bitWidth   = 16 := by rfl
+@[simp] theorem IScalarTy.I32_bitWidth_eq   : I32.bitWidth   = 32 := by rfl
+@[simp] theorem IScalarTy.I64_bitWidth_eq   : I64.bitWidth   = 64 := by rfl
+@[simp] theorem IScalarTy.I128_bitWidth_eq  : I128.bitWidth  = 128 := by rfl
+
+/-! The "normalized" bounds, that we use in practice -/
+def I8.min   : Int := -128
+def I8.max   : Int := 127
+def I16.min  : Int := -32768
+def I16.max  : Int := 32767
+def I32.min  : Int := -2147483648
+def I32.max  : Int := 2147483647
+def I64.min  : Int := -9223372036854775808
+def I64.max  : Int := 9223372036854775807
+def I128.min : Int := -170141183460469231731687303715884105728
+def I128.max : Int := 170141183460469231731687303715884105727
+
+def U8.max   : Nat := 255
+def U16.max  : Nat := 65535
+def U32.max  : Nat := 4294967295
+def U64.max  : Nat := 18446744073709551615
+def U128.max : Nat := 340282366920938463463374607431768211455
+
+/-! The "structured" bounds, expressed in terms of powers of two. -/
+
+def UScalar.smax (ty : UScalarTy) : ℕ := 2^ty.bitWidth - 1
+def IScalar.smin (ty : IScalarTy) : ℤ := -2^(ty.bitWidth - 1)
+def IScalar.smax (ty : IScalarTy) : ℤ := 2^(ty.bitWidth - 1) - 1
 
 def Isize.refined_min : { n:Int // n = I32.min ∨ n = I64.min } :=
-  ⟨ Isize.smin, by
-    simp [Isize.smin]
+  ⟨ IScalar.smin .Isize, by
+    simp [IScalar.smin]
     cases System.Platform.numBits_eq <;>
     unfold System.Platform.numBits at * <;> simp [*] <;> decide ⟩
 
 def Isize.refined_max : { n:Int // n = I32.max ∨ n = I64.max } :=
-  ⟨ Isize.smax, by
-    simp [Isize.smax]
+  ⟨ IScalar.smax .Isize, by
+    simp [IScalar.smax]
     cases System.Platform.numBits_eq <;>
     unfold System.Platform.numBits at * <;> simp [*] <;> decide ⟩
 
 def Usize.refined_max : { n:Nat // n = U32.max ∨ n = U64.max } :=
-  ⟨ Usize.smax, by
-    simp [Usize.smax]
+  ⟨ UScalar.smax .Usize, by
+    simp [UScalar.smax]
     cases System.Platform.numBits_eq <;>
     unfold System.Platform.numBits at * <;> simp [*] <;> decide ⟩
 
@@ -105,120 +126,19 @@ def Usize.max := Usize.refined_max.val
 
 theorem Usize.bounds_eq :
   Usize.max = U32.max ∨ Usize.max = U64.max := by
-  simp [Usize.min, Usize.max, refined_max, smin, smax]
+  simp [Usize.max, refined_max, UScalar.smax]
   cases System.Platform.numBits_eq <;>
   unfold System.Platform.numBits at * <;> simp [*] <;> decide
 
 theorem Isize.bounds_eq :
   (Isize.min = I32.min ∧ Isize.max = I32.max)
   ∨ (Isize.min = I64.min ∧ Isize.max = I64.max) := by
-  simp [Isize.min, Isize.max, refined_min, refined_max, smin, smax]
+  simp [Isize.min, Isize.max, refined_min, refined_max, IScalar.smin, IScalar.smax]
   cases System.Platform.numBits_eq <;>
   unfold System.Platform.numBits at * <;> simp [*] <;> decide
 
-inductive ScalarTy where
-| Isize
-| I8
-| I16
-| I32
-| I64
-| I128
-| Usize
-| U8
-| U16
-| U32
-| U64
-| U128
-
-@[reducible]
-def ScalarTy.isSigned (ty : ScalarTy) : Bool :=
+def UScalar.max (ty : UScalarTy) : Nat :=
   match ty with
-  | Isize
-  | I8
-  | I16
-  | I32
-  | I64
-  | I128 => true
-  | Usize
-  | U8
-  | U16
-  | U32
-  | U64
-  | U128 => false
-
--- FIXME(chore): bulk prove them via macro?
-instance : Fact (¬ ScalarTy.isSigned .Usize) where
-  out := by decide
-
-instance : Fact (¬ ScalarTy.isSigned .U8) where
-  out := by decide
-
-instance : Fact (¬ ScalarTy.isSigned .U16) where
-  out := by decide
-
-instance : Fact (¬ ScalarTy.isSigned .U32) where
-  out := by decide
-
-instance : Fact (¬ ScalarTy.isSigned .U64) where
-  out := by decide
-
-instance : Fact (¬ ScalarTy.isSigned .U128) where
-  out := by decide
-
-
-def Scalar.smin (ty : ScalarTy) : Int :=
-  match ty with
-  | .Isize => Isize.smin
-  | .I8    => I8.smin
-  | .I16   => I16.smin
-  | .I32   => I32.smin
-  | .I64   => I64.smin
-  | .I128  => I128.smin
-  | .Usize => Usize.smin
-  | .U8    => U8.smin
-  | .U16   => U16.smin
-  | .U32   => U32.smin
-  | .U64   => U64.smin
-  | .U128  => U128.smin
-
-def Scalar.smax (ty : ScalarTy) : Int :=
-  match ty with
-  | .Isize => Isize.smax
-  | .I8    => I8.smax
-  | .I16   => I16.smax
-  | .I32   => I32.smax
-  | .I64   => I64.smax
-  | .I128  => I128.smax
-  | .Usize => Usize.smax
-  | .U8    => U8.smax
-  | .U16   => U16.smax
-  | .U32   => U32.smax
-  | .U64   => U64.smax
-  | .U128  => U128.smax
-
-def Scalar.min (ty : ScalarTy) : Int :=
-  match ty with
-  | .Isize => Isize.min
-  | .I8    => I8.min
-  | .I16   => I16.min
-  | .I32   => I32.min
-  | .I64   => I64.min
-  | .I128  => I128.min
-  | .Usize => Usize.min
-  | .U8    => U8.min
-  | .U16   => U16.min
-  | .U32   => U32.min
-  | .U64   => U64.min
-  | .U128  => U128.min
-
-def Scalar.max (ty : ScalarTy) : Int :=
-  match ty with
-  | .Isize => Isize.max
-  | .I8    => I8.max
-  | .I16   => I16.max
-  | .I32   => I32.max
-  | .I64   => I64.max
-  | .I128  => I128.max
   | .Usize => Usize.max
   | .U8    => U8.max
   | .U16   => U16.max
@@ -226,112 +146,201 @@ def Scalar.max (ty : ScalarTy) : Int :=
   | .U64   => U64.max
   | .U128  => U128.max
 
-def Scalar.smin_eq (ty : ScalarTy) : Scalar.min ty = Scalar.smin ty := by
-  cases ty <;> rfl
-
-def Scalar.smax_eq (ty : ScalarTy) : Scalar.max ty = Scalar.smax ty := by
-  cases ty <;> rfl
-
--- "Conservative" bounds
--- We use those because we can't compare to the isize bounds (which can't
--- reduce at compile-time). Whenever we perform an arithmetic operation like
--- addition we need to check that the result is in bounds: we first compare
--- to the conservative bounds, which reduce, then compare to the real bounds.
--- This is useful for the various #asserts that we want to reduce at
--- type-checking time.
-def Scalar.cMin (ty : ScalarTy) : Int :=
+def IScalar.min (ty : IScalarTy) : Int :=
   match ty with
-  | .Isize => Scalar.min .I32
-  | _ => Scalar.min ty
+  | .Isize => Isize.min
+  | .I8    => I8.min
+  | .I16   => I16.min
+  | .I32   => I32.min
+  | .I64   => I64.min
+  | .I128  => I128.min
 
-def Scalar.cMax (ty : ScalarTy) : Int :=
+def IScalar.max (ty : IScalarTy) : Int :=
   match ty with
-  | .Isize => Scalar.max .I32
-  | .Usize => Scalar.max .U32
-  | _ => Scalar.max ty
+  | .Isize => Isize.max
+  | .I8    => I8.max
+  | .I16   => I16.max
+  | .I32   => I32.max
+  | .I64   => I64.max
+  | .I128  => I128.max
 
-theorem Scalar.min_lt_max (ty : ScalarTy) : Scalar.min ty < Scalar.max ty := by
-  cases ty <;> simp [Scalar.min, Scalar.max] <;> try decide
-  . simp [Isize.min, Isize.max]
-    have h1 := Isize.refined_min.property
-    have h2 := Isize.refined_max.property
-    cases h1 <;> cases h2 <;> simp [*] <;> decide
-  . simp [Usize.max]
-    have h := Usize.refined_max.property
-    cases h <;> simp [*] <;> decide
+def UScalar.smax_eq (ty : UScalarTy) : UScalar.max ty = UScalar.smax ty := by cases ty <;> rfl
+def IScalar.smin_eq (ty : IScalarTy) : IScalar.min ty = IScalar.smin ty := by cases ty <;> rfl
+def IScalar.smax_eq (ty : IScalarTy) : IScalar.max ty = IScalar.smax ty := by cases ty <;> rfl
 
-theorem Scalar.min_le_max (ty : ScalarTy) : Scalar.min ty ≤ Scalar.max ty := by
-  have := Scalar.min_lt_max ty
+theorem UScalar.bounds_eq (ty : UScalarTy) : UScalar.max ty = UScalar.smax ty := by
+  dcases ty <;> rfl
+
+theorem IScalar.bounds_eq (ty : IScalarTy) : IScalar.min ty = IScalar.smin ty ∧ IScalar.max ty = IScalar.smax ty := by
+  dcases ty <;> split_conjs <;> rfl
+
+/-
+"Conservative" bounds
+
+We use those because we can't compare to the isize bounds (which can't
+reduce at compile-time). Whenever we perform an arithmetic operation like
+addition we need to check that the result is in bounds: we first compare
+to the conservative bounds, which reduce, then compare to the real bounds.
+This is useful for the various #asserts that we want to reduce at
+type-checking time. -/
+
+def UScalar.cMax (ty : UScalarTy) : Int :=
+  match ty with
+  | .Usize => UScalar.max .U32
+  | _ => UScalar.max ty
+
+def IScalar.cMin (ty : IScalarTy) : Int :=
+  match ty with
+  | .Isize => IScalar.min .I32
+  | _ => IScalar.min ty
+
+def IScalar.cMax (ty : IScalarTy) : Int :=
+  match ty with
+  | .Isize => IScalar.max .I32
+  | _ => IScalar.max ty
+
+theorem UScalar.cMax_bound ty : UScalar.cMax ty ≤ UScalar.max ty := by
+  cases ty <;> (simp [UScalar.max, UScalar.cMax] at *; try decide)
+  have h := Usize.refined_max.property
+  cases h <;> simp [*, Usize.max]; decide
+
+theorem UScalar.cMax_suffices ty (h : x ≤ UScalar.cMax ty) : x ≤ UScalar.max ty := by
+  have := UScalar.cMax_bound ty
+  omega
+
+theorem IScalar.min_lt_max (ty : IScalarTy) : IScalar.min ty < IScalar.max ty := by
+  cases ty <;> simp [IScalar.min, IScalar.max] <;> try decide
+  simp [Isize.min, Isize.max]
+  have h1 := Isize.refined_min.property
+  have h2 := Isize.refined_max.property
+  cases h1 <;> cases h2 <;> simp [*] <;> decide
+
+theorem IScalar.min_le_max (ty : IScalarTy) : IScalar.min ty ≤ IScalar.max ty := by
+  have := IScalar.min_lt_max ty
   int_tac
 
-theorem Scalar.cMin_bound ty : Scalar.min ty ≤ Scalar.cMin ty := by
-  cases ty <;> (simp [Scalar.min, Scalar.max, Scalar.cMin, Scalar.cMax] at *; try decide)
+theorem IScalar.cMin_bound ty : IScalar.min ty ≤ IScalar.cMin ty := by
+  cases ty <;> (simp [IScalar.min, IScalar.max, IScalar.cMin, IScalar.cMax] at *; try decide)
   have h := Isize.refined_min.property
   cases h <;> simp [*, Isize.min]
   decide
 
-theorem Scalar.cMax_bound ty : Scalar.cMax ty ≤ Scalar.max ty := by
-  cases ty <;> (simp [Scalar.min, Scalar.max, Scalar.cMin, Scalar.cMax] at *; try decide)
-  . have h := Isize.refined_max.property
-    cases h <;> simp [*, Isize.max]; decide
-  . have h := Usize.refined_max.property
-    cases h <;> simp [*, Usize.max]; decide
+theorem IScalar.cMax_bound ty : IScalar.cMax ty ≤ IScalar.max ty := by
+  cases ty <;> (simp [IScalar.min, IScalar.max, IScalar.cMin, IScalar.cMax] at *; try decide)
+  have h := Isize.refined_max.property
+  cases h <;> simp [*, Isize.max]; decide
 
-theorem Scalar.cMin_suffices ty (h : Scalar.cMin ty ≤ x) : Scalar.min ty ≤ x := by
-  have := Scalar.cMin_bound ty
+theorem IScalar.cMin_suffices ty (h : IScalar.cMin ty ≤ x) : IScalar.min ty ≤ x := by
+  have := IScalar.cMin_bound ty
   omega
 
-theorem Scalar.cMax_suffices ty (h : x ≤ Scalar.cMax ty) : x ≤ Scalar.max ty := by
-  have := Scalar.cMax_bound ty
+theorem IScalar.cMax_suffices ty (h : x ≤ IScalar.cMax ty) : x ≤ IScalar.max ty := by
+  have := IScalar.cMax_bound ty
   omega
 
-/-- The scalar type.
+/-- The unsigned scalar type.
 
-    We could use a subtype, but it using a custom structure type allows us
-    to have more control over the coercions and the simplifications (we tried
-    using a subtype and it caused issues especially as we had to make the Scalar
-    type non-reducible, so that we could have more control, but leading to
-    some natural equalities not being obvious to the simplifier anymore).
- -/
-structure Scalar (ty : ScalarTy) where
-  val : Int
-  hmin : Scalar.min ty ≤ val
-  hmax : val ≤ Scalar.max ty
+    Underneath, we simply use a bit-vector.
+-/
+structure UScalar (ty : UScalarTy) where
+  bv : BitVec ty.bitWidth
 deriving Repr, BEq, DecidableEq
 
-instance {ty} : BEq (Scalar ty) where
-  beq a b := a.val = b.val
+def UScalar.val {ty} (x : UScalar ty) : ℕ := x.bv.toNat
 
-instance {ty} : LawfulBEq (Scalar ty) where
+def UScalar.hBounds {ty} (x : UScalar ty) : x.val ≤ UScalar.max ty := by
+  dcases h: x.bv
+  simp [h, val, bounds_eq, smax]
+  omega
+
+def UScalar.hmax {ty} (x : UScalar ty) : x.val ≤ UScalar.max ty := x.hBounds
+
+/-- The signed scalar type.
+
+    Underneath, we simply use a bit-vector.
+ -/
+structure IScalar (ty : IScalarTy) where
+  bv : BitVec ty.bitWidth
+deriving Repr, BEq, DecidableEq
+
+def IScalar.val {ty} (x : IScalar ty) : ℤ := x.bv.toInt
+
+def IScalar.hBounds {ty} (x : IScalar ty) : IScalar.min ty ≤ x.val ∧ x.val ≤ IScalar.max ty := by
+  match x with
+  | ⟨ ⟨ fin ⟩ ⟩ =>
+    simp [val, bounds_eq, smin, smax, BitVec.toInt]
+    dcases ty <;> simp at * <;> try omega
+    have hFinLt := fin.isLt
+    cases h: System.Platform.numBits_eq <;> simp_all only [IScalarTy.Isize_bitWidth_eq,
+      size_num_bits, true_or, Nat.add_one_sub_one] <;>
+    omega
+
+def IScalar.hmin {ty} (x : IScalar ty) : IScalar.min ty ≤ x.val := x.hBounds.left
+def IScalar.hmax {ty} (x : IScalar ty) : x.val ≤ IScalar.max ty  := x.hBounds.right
+
+instance {ty} : BEq (UScalar ty) where
+  beq a b := a.bv = b.bv
+
+instance {ty} : BEq (IScalar ty) where
+  beq a b := a.bv = b.bv
+
+instance {ty} : LawfulBEq (UScalar ty) where
+  eq_of_beq {a b} := by cases a; cases b; simp [BEq.beq]
+  rfl {a} := by cases a; simp [BEq.beq]
+
+instance {ty} : LawfulBEq (IScalar ty) where
   eq_of_beq {a b} := by cases a; cases b; simp[BEq.beq]
   rfl {a} := by cases a; simp [BEq.beq]
 
-instance (ty : ScalarTy) : CoeOut (Scalar ty) Int where
+instance (ty : UScalarTy) : CoeOut (UScalar ty) Nat where
+  coe := λ v => v.val
+
+instance (ty : IScalarTy) : CoeOut (IScalar ty) Int where
   coe := λ v => v.val
 
 /- Activate the ↑ notation -/
-attribute [coe] Scalar.val
+attribute [coe] UScalar.val IScalar.val
 
-theorem Scalar.bound_suffices (ty : ScalarTy) (x : Int) :
-  Scalar.cMin ty ≤ x ∧ x ≤ Scalar.cMax ty ->
-  Scalar.min ty ≤ x ∧ x ≤ Scalar.max ty
+theorem IScalar.bound_suffices (ty : IScalarTy) (x : Int) :
+  IScalar.cMin ty ≤ x ∧ x ≤ IScalar.cMax ty ->
+  IScalar.min ty ≤ x ∧ x ≤ IScalar.max ty
   :=
   λ h => by
-  apply And.intro <;> have hmin := Scalar.cMin_bound ty <;> have hmax := Scalar.cMax_bound ty <;> omega
+  apply And.intro <;> have hmin := IScalar.cMin_bound ty <;> have hmax := IScalar.cMax_bound ty <;> omega
 
-def Scalar.ofIntCore {ty : ScalarTy} (x : Int)
-  (h : Scalar.min ty ≤ x ∧ x ≤ Scalar.max ty) : Scalar ty :=
-  { val := x, hmin := h.left, hmax := h.right }
+theorem UScalar.bound_suffices (ty : UScalarTy) (x : Nat) :
+  x ≤ UScalar.cMax ty -> x ≤ UScalar.max ty
+  :=
+  λ h => by have hmax := UScalar.cMax_bound ty; omega
 
-@[reducible] def Scalar.ofInt {ty : ScalarTy} (x : Int)
-  (hInBounds : Scalar.cMin ty ≤ x ∧ x ≤ Scalar.cMax ty := by decide) : Scalar ty :=
-  Scalar.ofIntCore x (Scalar.bound_suffices ty x hInBounds)
+/- TODO: remove? Having a check on the bounds is a good sanity check, and it allows to prove
+   nice theorems like `(ofIntCore x ..).val = x`, though `BitVec` also has powerful simplification lemmas. -/
+def UScalar.ofNatCore {ty : UScalarTy} (x : Nat) (_ : x ≤ UScalar.max ty) : UScalar ty :=
+  { bv := BitVec.ofNat _ x }
 
-@[simp] abbrev Scalar.in_bounds (ty : ScalarTy) (x : Int) : Prop :=
-  Scalar.min ty ≤ x ∧ x ≤ Scalar.max ty
+-- TODO: remove?
+def IScalar.ofIntCore {ty : IScalarTy} (x : Int) (_ : IScalar.min ty ≤ x ∧ x ≤ IScalar.max ty) : IScalar ty :=
+  { bv := BitVec.ofInt _ x }
 
-@[simp] abbrev Scalar.check_bounds (ty : ScalarTy) (x : Int) : Bool :=
-  (Scalar.cMin ty ≤ x || Scalar.min ty ≤ x) ∧ (x ≤ Scalar.cMax ty || x ≤ Scalar.max ty)
+@[reducible] def UScalar.ofNat {ty : UScalarTy} (x : Nat)
+  (hInBounds : x ≤ UScalar.cMax ty := by decide) : UScalar ty :=
+  UScalar.ofNatCore x (UScalar.bound_suffices ty x hInBounds)
+
+@[reducible] def IScalar.ofInt {ty : IScalarTy} (x : Int)
+  (hInBounds : IScalar.cMin ty ≤ x ∧ x ≤ IScalar.cMax ty := by decide) : IScalar ty :=
+  IScalar.ofIntCore x (IScalar.bound_suffices ty x hInBounds)
+
+@[simp] abbrev UScalar.inBounds (ty : UScalarTy) (x : Nat) : Prop :=
+  x ≤ UScalar.max ty
+
+@[simp] abbrev IScalar.inBounds (ty : IScalarTy) (x : Int) : Prop :=
+  IScalar.min ty ≤ x ∧ x ≤ IScalar.max ty
+
+@[simp] abbrev UScalar.check_bounds (ty : UScalarTy) (x : Nat) : Bool :=
+  x ≤ UScalar.cMax ty || x ≤ UScalar.max ty
+
+@[simp] abbrev IScalar.check_bounds (ty : IScalarTy) (x : Int) : Bool :=
+  (IScalar.cMin ty ≤ x || IScalar.min ty ≤ x) ∧ (x ≤ IScalar.cMax ty || x ≤ IScalar.max ty)
 
 /- Discussion:
    This coercion can be slightly annoying at times, because if we write
@@ -345,287 +354,414 @@ instance {ty: ScalarTy} [InBounds ty (Int.ofNat n)]: OfNat (Scalar ty) (n: ℕ) 
   ofNat := Scalar.ofInt n
 -/
 
-theorem Scalar.check_bounds_imp_in_bounds {ty : ScalarTy} {x : Int}
-  (h: Scalar.check_bounds ty x) :
-  Scalar.in_bounds ty x := by
+theorem UScalar.check_bounds_imp_inBounds {ty : UScalarTy} {x : Nat}
+  (h: UScalar.check_bounds ty x) :
+  UScalar.inBounds ty x := by
   simp at *
-  have ⟨ hmin, hmax ⟩ := h
-  have hbmin := Scalar.cMin_bound ty
-  have hbmax := Scalar.cMax_bound ty
-  cases hmin <;> cases hmax <;> apply And.intro <;> omega
+  have hbmax := UScalar.cMax_bound ty
+  cases h <;> omega
 
-theorem Scalar.check_bounds_eq_in_bounds (ty : ScalarTy) (x : Int) :
-  Scalar.check_bounds ty x ↔ Scalar.in_bounds ty x := by
+theorem UScalar.check_bounds_eq_inBounds (ty : UScalarTy) (x : Nat) :
+  UScalar.check_bounds ty x ↔ UScalar.inBounds ty x := by
   constructor <;> intro h
-  . apply (check_bounds_imp_in_bounds h)
+  . apply (check_bounds_imp_inBounds h)
   . simp_all
 
--- Further thoughts: look at what has been done here:
--- https://github.com/leanprover-community/mathlib4/blob/master/Mathlib/Data/Fin/Basic.lean
--- and
--- https://github.com/leanprover-community/mathlib4/blob/master/Mathlib/Data/UInt.lean
--- which both contain a fair amount of reasoning already!
-def Scalar.tryMkOpt (ty : ScalarTy) (x : Int) : Option (Scalar ty) :=
-  if h:Scalar.check_bounds ty x then
-    -- If we do:
-    -- ```
-    -- let ⟨ hmin, hmax ⟩ := (Scalar.check_bounds_imp_in_bounds h)
-    -- Scalar.ofIntCore x hmin hmax
-    -- ```
-    -- then normalization blocks (for instance, some proofs which use reflexivity fail).
-    -- However, the version below doesn't block reduction (TODO: investigate):
-    some (Scalar.ofIntCore x (Scalar.check_bounds_imp_in_bounds h))
+theorem IScalar.check_bounds_imp_inBounds {ty : IScalarTy} {x : Int}
+  (h: IScalar.check_bounds ty x) :
+  IScalar.inBounds ty x := by
+  simp at *
+  have ⟨ hmin, hmax ⟩ := h
+  have hbmin := IScalar.cMin_bound ty
+  have hbmax := IScalar.cMax_bound ty
+  cases hmin <;> cases hmax <;> apply And.intro <;> omega
+
+theorem IScalar.check_bounds_eq_inBounds (ty : IScalarTy) (x : Int) :
+  IScalar.check_bounds ty x ↔ IScalar.inBounds ty x := by
+  constructor <;> intro h
+  . apply (check_bounds_imp_inBounds h)
+  . simp_all
+
+def UScalar.tryMkOpt (ty : UScalarTy) (x : Nat) : Option (UScalar ty) :=
+  if h:UScalar.check_bounds ty x then
+    some (UScalar.ofNatCore x (UScalar.check_bounds_imp_inBounds h))
   else none
 
-def Scalar.tryMk (ty : ScalarTy) (x : Int) : Result (Scalar ty) :=
+def UScalar.tryMk (ty : UScalarTy) (x : Nat) : Result (UScalar ty) :=
   Result.ofOption (tryMkOpt ty x) integerOverflow
 
-theorem Scalar.tryMk_eq (ty : ScalarTy) (x : Int) :
-  match tryMk ty x with
-  | ok y => y.val = x ∧ in_bounds ty x
-  | fail _ => ¬ (in_bounds ty x)
-  | _ => False := by
-  simp [tryMk, ofOption, tryMkOpt, ofIntCore]
-  have h := check_bounds_eq_in_bounds ty x
-  split_ifs <;> simp_all
+def IScalar.tryMkOpt (ty : IScalarTy) (x : Int) : Option (IScalar ty) :=
+  if h:IScalar.check_bounds ty x then
+    some (IScalar.ofIntCore x (IScalar.check_bounds_imp_inBounds h))
+  else none
 
-@[simp] theorem Scalar.tryMk_eq_div (ty : ScalarTy) (x : Int) :
+def IScalar.tryMk (ty : IScalarTy) (x : Int) : Result (IScalar ty) :=
+  Result.ofOption (tryMkOpt ty x) integerOverflow
+
+theorem UScalar.tryMk_eq (ty : UScalarTy) (x : Nat) :
+  match tryMk ty x with
+  | ok y => y.val = x ∧ inBounds ty x
+  | fail _ => ¬ (inBounds ty x)
+  | _ => False := by
+  simp [tryMk, ofOption, tryMkOpt, ofNatCore]
+  have h := check_bounds_eq_inBounds ty x
+  split_ifs <;> simp_all
+  simp [UScalar.val, UScalarTy.bitWidth, max] at *
+  dcases ty <;> simp_all [U8.max, U16.max, U32.max, U64.max, U128.max, Usize.max, Usize.refined_max, smax] <;> try omega
+  cases h: System.Platform.numBits_eq <;> simp_all <;> omega
+
+@[simp] theorem UScalar.tryMk_eq_div (ty : UScalarTy) (x : Nat) :
   tryMk ty x = div ↔ False := by
   simp [tryMk, ofOption, tryMkOpt]
   split_ifs <;> simp
 
-@[simp] theorem zero_in_cbounds {ty : ScalarTy} : Scalar.cMin ty ≤ 0 ∧ 0 ≤ Scalar.cMax ty := by
-  cases ty <;> simp [Scalar.cMax, Scalar.cMin, Scalar.max, Scalar.min] <;> decide
+theorem IScalar.tryMk_eq (ty : IScalarTy) (x : Int) :
+  match tryMk ty x with
+  | ok y => y.val = x ∧ inBounds ty x
+  | fail _ => ¬ (inBounds ty x)
+  | _ => False := by
+  simp [tryMk, ofOption, tryMkOpt, ofIntCore]
+  have h := check_bounds_eq_inBounds ty x
+  split_ifs <;> simp_all
+  simp [IScalar.val, IScalarTy.bitWidth, min, max] at *
+  dcases ty <;>
+  simp_all [I8.min, I16.min, I32.min, I64.min, I128.min, Isize.min,
+            I8.max, I16.max, I32.max, I64.max, I128.max, Isize.max,
+            Isize.refined_min, smin, Isize.refined_max, smax] <;>
+  simp [Int.bmod] <;> split <;> (try omega) <;>
+  cases h: System.Platform.numBits_eq <;> simp_all <;> omega
 
--- The scalar types
--- We declare the definitions as reducible so that Lean can unfold them (useful
--- for type class resolution for instance).
-@[reducible] def Isize := Scalar .Isize
-@[reducible] def I8    := Scalar .I8
-@[reducible] def I16   := Scalar .I16
-@[reducible] def I32   := Scalar .I32
-@[reducible] def I64   := Scalar .I64
-@[reducible] def I128  := Scalar .I128
-@[reducible] def Usize := Scalar .Usize
-@[reducible] def U8    := Scalar .U8
-@[reducible] def U16   := Scalar .U16
-@[reducible] def U32   := Scalar .U32
-@[reducible] def U64   := Scalar .U64
-@[reducible] def U128  := Scalar .U128
+@[simp] theorem IScalar.tryMk_eq_div (ty : IScalarTy) (x : Int) :
+  tryMk ty x = div ↔ False := by
+  simp [tryMk, ofOption, tryMkOpt]
+  split_ifs <;> simp
 
--- ofIntCore
+@[simp] theorem UScalar.zero_in_cbounds {ty : UScalarTy} : 0 ≤ UScalar.cMax ty := by
+  cases ty <;> simp [UScalar.cMax, UScalar.max]
+
+@[simp] theorem IScalar.zero_in_cbounds {ty : IScalarTy} : IScalar.cMin ty ≤ 0 ∧ 0 ≤ IScalar.cMax ty := by
+  cases ty <;> simp [IScalar.cMax, IScalar.cMin, IScalar.max, IScalar.min] <;> decide
+
+/-! The scalar types. -/
+@[reducible] def Usize := UScalar .Usize
+@[reducible] def U8    := UScalar .U8
+@[reducible] def U16   := UScalar .U16
+@[reducible] def U32   := UScalar .U32
+@[reducible] def U64   := UScalar .U64
+@[reducible] def U128  := UScalar .U128
+@[reducible] def Isize := IScalar .Isize
+@[reducible] def I8    := IScalar .I8
+@[reducible] def I16   := IScalar .I16
+@[reducible] def I32   := IScalar .I32
+@[reducible] def I64   := IScalar .I64
+@[reducible] def I128  := IScalar .I128
+
+/-!  ofNatCore -/
 -- TODO: typeclass?
-def Isize.ofIntCore := @Scalar.ofIntCore .Isize
-def I8.ofIntCore    := @Scalar.ofIntCore .I8
-def I16.ofIntCore   := @Scalar.ofIntCore .I16
-def I32.ofIntCore   := @Scalar.ofIntCore .I32
-def I64.ofIntCore   := @Scalar.ofIntCore .I64
-def I128.ofIntCore  := @Scalar.ofIntCore .I128
-def Usize.ofIntCore := @Scalar.ofIntCore .Usize
-def U8.ofIntCore    := @Scalar.ofIntCore .U8
-def U16.ofIntCore   := @Scalar.ofIntCore .U16
-def U32.ofIntCore   := @Scalar.ofIntCore .U32
-def U64.ofIntCore   := @Scalar.ofIntCore .U64
-def U128.ofIntCore  := @Scalar.ofIntCore .U128
+def Usize.ofNatCore := @UScalar.ofNatCore .Usize
+def U8.ofNatCore    := @UScalar.ofNatCore .U8
+def U16.ofNatCore   := @UScalar.ofNatCore .U16
+def U32.ofNatCore   := @UScalar.ofNatCore .U32
+def U64.ofNatCore   := @UScalar.ofNatCore .U64
+def U128.ofNatCore  := @UScalar.ofNatCore .U128
 
---  ofInt
+/-!  ofIntCore -/
+def Isize.ofIntCore := @IScalar.ofIntCore .Isize
+def I8.ofIntCore    := @IScalar.ofIntCore .I8
+def I16.ofIntCore   := @IScalar.ofIntCore .I16
+def I32.ofIntCore   := @IScalar.ofIntCore .I32
+def I64.ofIntCore   := @IScalar.ofIntCore .I64
+def I128.ofIntCore  := @IScalar.ofIntCore .I128
+
+/-!  ofNat -/
 -- TODO: typeclass?
-abbrev Isize.ofInt := @Scalar.ofInt .Isize
-abbrev I8.ofInt    := @Scalar.ofInt .I8
-abbrev I16.ofInt   := @Scalar.ofInt .I16
-abbrev I32.ofInt   := @Scalar.ofInt .I32
-abbrev I64.ofInt   := @Scalar.ofInt .I64
-abbrev I128.ofInt  := @Scalar.ofInt .I128
-abbrev Usize.ofInt := @Scalar.ofInt .Usize
-abbrev U8.ofInt    := @Scalar.ofInt .U8
-abbrev U16.ofInt   := @Scalar.ofInt .U16
-abbrev U32.ofInt   := @Scalar.ofInt .U32
-abbrev U64.ofInt   := @Scalar.ofInt .U64
-abbrev U128.ofInt  := @Scalar.ofInt .U128
+abbrev Usize.ofNat := @UScalar.ofNat .Usize
+abbrev U8.ofNat    := @UScalar.ofNat .U8
+abbrev U16.ofNat   := @UScalar.ofNat .U16
+abbrev U32.ofNat   := @UScalar.ofNat .U32
+abbrev U64.ofNat   := @UScalar.ofNat .U64
+abbrev U128.ofNat  := @UScalar.ofNat .U128
 
--- TODO: factor those lemmas out
-@[simp] theorem Scalar.ofInt_val_eq {ty} (h : Scalar.min ty ≤ x ∧ x ≤ Scalar.max ty) : (Scalar.ofIntCore x h).val = x := by
-  simp [Scalar.ofInt, Scalar.ofIntCore]
+/-!  ofInt -/
+abbrev Isize.ofInt := @IScalar.ofInt .Isize
+abbrev I8.ofInt    := @IScalar.ofInt .I8
+abbrev I16.ofInt   := @IScalar.ofInt .I16
+abbrev I32.ofInt   := @IScalar.ofInt .I32
+abbrev I64.ofInt   := @IScalar.ofInt .I64
+abbrev I128.ofInt  := @IScalar.ofInt .I128
 
-@[simp] theorem Isize.ofInt_val_eq (h : Scalar.min ScalarTy.Isize ≤ x ∧ x ≤ Scalar.max ScalarTy.Isize) : (Isize.ofIntCore x h).val = x := by
-  apply Scalar.ofInt_val_eq h
+@[simp] theorem UScalar.ofNat_val_eq {ty} (h : x ≤ UScalar.max ty) : (UScalar.ofNatCore x h).val = x := by
+  simp [UScalar.ofNat, UScalar.ofNatCore, UScalar.val, max]
+  dcases ty <;> simp_all [U8.max, U16.max, U32.max, U64.max, U128.max, Usize.max, Usize.refined_max, smax, max] <;> try omega
+  cases h: System.Platform.numBits_eq <;> simp_all <;> omega
 
-@[simp] theorem I8.ofInt_val_eq (h : Scalar.min ScalarTy.I8 ≤ x ∧ x ≤ Scalar.max ScalarTy.I8) : (I8.ofIntCore x h).val = x := by
-  apply Scalar.ofInt_val_eq h
+@[simp] theorem Usize.ofNat_val_eq (h : x ≤ UScalar.max UScalarTy.Usize) : (Usize.ofNatCore x h).val = x := by
+  apply UScalar.ofNat_val_eq h
 
-@[simp] theorem I16.ofInt_val_eq (h : Scalar.min ScalarTy.I16 ≤ x ∧ x ≤ Scalar.max ScalarTy.I16) : (I16.ofIntCore x h).val = x := by
-  apply Scalar.ofInt_val_eq h
+@[simp] theorem U8.ofNat_val_eq (h : x ≤ UScalar.max UScalarTy.U8) : (U8.ofNatCore x h).val = x := by
+  apply UScalar.ofNat_val_eq h
 
-@[simp] theorem I32.ofInt_val_eq (h : Scalar.min ScalarTy.I32 ≤ x ∧ x ≤ Scalar.max ScalarTy.I32) : (I32.ofIntCore x h).val = x := by
-  apply Scalar.ofInt_val_eq h
+@[simp] theorem U16.ofNat_val_eq (h : x ≤ UScalar.max UScalarTy.U16) : (U16.ofNatCore x h).val = x := by
+  apply UScalar.ofNat_val_eq h
 
-@[simp] theorem I64.ofInt_val_eq (h : Scalar.min ScalarTy.I64 ≤ x ∧ x ≤ Scalar.max ScalarTy.I64) : (I64.ofIntCore x h).val = x := by
-  apply Scalar.ofInt_val_eq h
+@[simp] theorem U32.ofNat_val_eq (h : x ≤ UScalar.max UScalarTy.U32) : (U32.ofNatCore x h).val = x := by
+  apply UScalar.ofNat_val_eq h
 
-@[simp] theorem I128.ofInt_val_eq (h : Scalar.min ScalarTy.I128 ≤ x ∧ x ≤ Scalar.max ScalarTy.I128) : (I128.ofIntCore x h).val = x := by
-  apply Scalar.ofInt_val_eq h
+@[simp] theorem U64.ofNat_val_eq (h : x ≤ UScalar.max UScalarTy.U64) : (U64.ofNatCore x h).val = x := by
+  apply UScalar.ofNat_val_eq h
 
-@[simp] theorem Usize.ofInt_val_eq (h : Scalar.min ScalarTy.Usize ≤ x ∧ x ≤ Scalar.max ScalarTy.Usize) : (Usize.ofIntCore x h).val = x := by
-  apply Scalar.ofInt_val_eq h
+@[simp] theorem U128.ofNat_val_eq (h : x ≤ UScalar.max UScalarTy.U128) : (U128.ofNatCore x h).val = x := by
+  apply UScalar.ofNat_val_eq h
 
-@[simp] theorem U8.ofInt_val_eq (h : Scalar.min ScalarTy.U8 ≤ x ∧ x ≤ Scalar.max ScalarTy.U8) : (U8.ofIntCore x h).val = x := by
-  apply Scalar.ofInt_val_eq h
+@[simp] theorem IScalar.ofInt_val_eq {ty} (h : IScalar.min ty ≤ x ∧ x ≤ IScalar.max ty) : (IScalar.ofIntCore x h).val = x := by
+  simp [IScalar.ofInt, IScalar.ofIntCore, IScalar.val, min, max]
+  dcases ty <;>
+  simp_all [I8.min, I16.min, I32.min, I64.min, I128.min, Isize.min,
+            I8.max, I16.max, I32.max, I64.max, I128.max, Isize.max,
+            Isize.refined_min, smin, Isize.refined_max, smax, min, max] <;>
+  simp [Int.bmod] <;> split <;> (try omega) <;>
+  cases h: System.Platform.numBits_eq <;> simp_all <;> omega
 
-@[simp] theorem U16.ofInt_val_eq (h : Scalar.min ScalarTy.U16 ≤ x ∧ x ≤ Scalar.max ScalarTy.U16) : (U16.ofIntCore x h).val = x := by
-  apply Scalar.ofInt_val_eq h
+@[simp] theorem Isize.ofInt_val_eq (h : IScalar.min IScalarTy.Isize ≤ x ∧ x ≤ IScalar.max IScalarTy.Isize) : (Isize.ofIntCore x h).val = x := by
+  apply IScalar.ofInt_val_eq h
 
-@[simp] theorem U32.ofInt_val_eq (h : Scalar.min ScalarTy.U32 ≤ x ∧ x ≤ Scalar.max ScalarTy.U32) : (U32.ofIntCore x h).val = x := by
-  apply Scalar.ofInt_val_eq h
+@[simp] theorem I8.ofInt_val_eq (h : IScalar.min IScalarTy.I8 ≤ x ∧ x ≤ IScalar.max IScalarTy.I8) : (I8.ofIntCore x h).val = x := by
+  apply IScalar.ofInt_val_eq h
 
-@[simp] theorem U64.ofInt_val_eq (h : Scalar.min ScalarTy.U64 ≤ x ∧ x ≤ Scalar.max ScalarTy.U64) : (U64.ofIntCore x h).val = x := by
-  apply Scalar.ofInt_val_eq h
+@[simp] theorem I16.ofInt_val_eq (h : IScalar.min IScalarTy.I16 ≤ x ∧ x ≤ IScalar.max IScalarTy.I16) : (I16.ofIntCore x h).val = x := by
+  apply IScalar.ofInt_val_eq h
 
-@[simp] theorem U128.ofInt_val_eq (h : Scalar.min ScalarTy.U128 ≤ x ∧ x ≤ Scalar.max ScalarTy.U128) : (U128.ofIntCore x h).val = x := by
-  apply Scalar.ofInt_val_eq h
+@[simp] theorem I32.ofInt_val_eq (h : IScalar.min IScalarTy.I32 ≤ x ∧ x ≤ IScalar.max IScalarTy.I32) : (I32.ofIntCore x h).val = x := by
+  apply IScalar.ofInt_val_eq h
 
-instance (ty : ScalarTy) : Inhabited (Scalar ty) := by
-  constructor; cases ty <;> apply (Scalar.ofInt 0)
+@[simp] theorem I64.ofInt_val_eq (h : IScalar.min IScalarTy.I64 ≤ x ∧ x ≤ IScalar.max IScalarTy.I64) : (I64.ofIntCore x h).val = x := by
+  apply IScalar.ofInt_val_eq h
 
--- TODO: reducible?
-@[reducible] def core_isize_min : Isize := Scalar.ofIntCore Isize.min (by simp [Scalar.min, Scalar.max]; apply (Scalar.min_le_max .Isize))
-@[reducible] def core_isize_max : Isize := Scalar.ofIntCore Isize.max (by simp [Scalar.min, Scalar.max]; apply (Scalar.min_le_max .Isize))
-@[reducible] def core_i8_min : I8 := Scalar.ofInt I8.min
-@[reducible] def core_i8_max : I8 := Scalar.ofInt I8.max
-@[reducible] def core_i16_min : I16 := Scalar.ofInt I16.min
-@[reducible] def core_i16_max : I16 := Scalar.ofInt I16.max
-@[reducible] def core_i32_min : I32 := Scalar.ofInt I32.min
-@[reducible] def core_i32_max : I32 := Scalar.ofInt I32.max
-@[reducible] def core_i64_min : I64 := Scalar.ofInt I64.min
-@[reducible] def core_i64_max : I64 := Scalar.ofInt I64.max
-@[reducible] def core_i128_min : I128 := Scalar.ofInt I128.min
-@[reducible] def core_i128_max : I128 := Scalar.ofInt I128.max
+@[simp] theorem I128.ofInt_val_eq (h : IScalar.min IScalarTy.I128 ≤ x ∧ x ≤ IScalar.max IScalarTy.I128) : (I128.ofIntCore x h).val = x := by
+  apply IScalar.ofInt_val_eq h
 
--- TODO: reducible?
-@[reducible] def core_usize_min : Usize := Scalar.ofIntCore Usize.min (by simp [Scalar.min, Scalar.max])
-@[reducible] def core_usize_max : Usize := Scalar.ofIntCore Usize.max (by simp [Scalar.min, Scalar.max])
-@[reducible] def core_u8_min : U8 := Scalar.ofInt U8.min
-@[reducible] def core_u8_max : U8 := Scalar.ofInt U8.max
-@[reducible] def core_u16_min : U16 := Scalar.ofInt U16.min
-@[reducible] def core_u16_max : U16 := Scalar.ofInt U16.max
-@[reducible] def core_u32_min : U32 := Scalar.ofInt U32.min
-@[reducible] def core_u32_max : U32 := Scalar.ofInt U32.max
-@[reducible] def core_u64_min : U64 := Scalar.ofInt U64.min
-@[reducible] def core_u64_max : U64 := Scalar.ofInt U64.max
-@[reducible] def core_u128_min : U128 := Scalar.ofInt U128.min
-@[reducible] def core_u128_max : U128 := Scalar.ofInt U128.max
+instance (ty : UScalarTy) : Inhabited (UScalar ty) := by
+  constructor; cases ty <;> apply (UScalar.ofNat 0)
 
--- Comparisons
-instance {ty} : LT (Scalar ty) where
+instance (ty : IScalarTy) : Inhabited (IScalar ty) := by
+  constructor; cases ty <;> apply (IScalar.ofInt 0)
+
+@[reducible] def core_usize_min : Usize := UScalar.ofNatCore 0 (by simp)
+@[reducible] def core_usize_max : Usize := UScalar.ofNatCore Usize.max (by simp [UScalar.max])
+@[reducible] def core_u8_min : U8 := UScalar.ofNat 0
+@[reducible] def core_u8_max : U8 := UScalar.ofNat U8.max
+@[reducible] def core_u16_min : U16 := UScalar.ofNat 0
+@[reducible] def core_u16_max : U16 := UScalar.ofNat U16.max
+@[reducible] def core_u32_min : U32 := UScalar.ofNat 0
+@[reducible] def core_u32_max : U32 := UScalar.ofNat U32.max
+@[reducible] def core_u64_min : U64 := UScalar.ofNat 0
+@[reducible] def core_u64_max : U64 := UScalar.ofNat U64.max
+@[reducible] def core_u128_min : U128 := UScalar.ofNat 0
+@[reducible] def core_u128_max : U128 := UScalar.ofNat U128.max
+
+@[reducible] def core_isize_min : Isize := IScalar.ofIntCore Isize.min (by simp [IScalar.min, IScalar.max]; apply (IScalar.min_le_max .Isize))
+@[reducible] def core_isize_max : Isize := IScalar.ofIntCore Isize.max (by simp [IScalar.min, IScalar.max]; apply (IScalar.min_le_max .Isize))
+@[reducible] def core_i8_min : I8 := IScalar.ofInt I8.min
+@[reducible] def core_i8_max : I8 := IScalar.ofInt I8.max
+@[reducible] def core_i16_min : I16 := IScalar.ofInt I16.min
+@[reducible] def core_i16_max : I16 := IScalar.ofInt I16.max
+@[reducible] def core_i32_min : I32 := IScalar.ofInt I32.min
+@[reducible] def core_i32_max : I32 := IScalar.ofInt I32.max
+@[reducible] def core_i64_min : I64 := IScalar.ofInt I64.min
+@[reducible] def core_i64_max : I64 := IScalar.ofInt I64.max
+@[reducible] def core_i128_min : I128 := IScalar.ofInt I128.min
+@[reducible] def core_i128_max : I128 := IScalar.ofInt I128.max
+
+/-! Comparisons -/
+instance {ty} : LT (UScalar ty) where
   lt a b := LT.lt a.val b.val
 
-instance {ty} : LE (Scalar ty) where le a b := LE.le a.val b.val
+instance {ty} : LE (UScalar ty) where le a b := LE.le a.val b.val
 
--- Not marking this one with @[simp] on purpose: if we have `x = y` somewhere in the context,
--- we may want to use it to substitute `y` with `x` somewhere.
-theorem Scalar.eq_equiv {ty : ScalarTy} (x y : Scalar ty) :
+instance {ty} : LT (IScalar ty) where
+  lt a b := LT.lt a.val b.val
+
+instance {ty} : LE (IScalar ty) where le a b := LE.le a.val b.val
+
+/- Not marking this one with @[simp] on purpose: if we have `x = y` somewhere in the context,
+   we may want to use it to substitute `y` with `x` somewhere. -/
+theorem UScalar.eq_equiv {ty : UScalarTy} (x y : UScalar ty) :
+  x = y ↔ (↑x : Nat) = ↑y := by
+  cases x; cases y; simp_all [UScalar.val, BitVec.toNat_eq]
+
+@[simp] theorem UScalar.eq_imp {ty : UScalarTy} (x y : UScalar ty) :
+  (↑x : Nat) = ↑y → x = y := (eq_equiv x y).mpr
+
+@[simp] theorem UScalar.lt_equiv {ty : UScalarTy} (x y : UScalar ty) :
+  x < y ↔ (↑x : Nat) < ↑y := by
+  rw [LT.lt, instLTUScalar]
+
+@[simp] theorem UScalar.lt_imp {ty : UScalarTy} (x y : UScalar ty) :
+  (↑x : Nat) < (↑y) → x < y := (lt_equiv x y).mpr
+
+@[simp] theorem UScalar.le_equiv {ty : UScalarTy} (x y : UScalar ty) :
+  x ≤ y ↔ (↑x : Nat) ≤ ↑y := by
+  rw [LE.le, instLEUScalar]
+
+@[simp] theorem UScalar.le_imp {ty : UScalarTy} (x y : UScalar ty) :
+  (↑x : Nat) ≤ ↑y → x ≤ y := (le_equiv x y).mpr
+
+theorem IScalar.eq_equiv {ty : IScalarTy} (x y : IScalar ty) :
   x = y ↔ (↑x : Int) = ↑y := by
-  cases x; cases y; simp_all
+  cases x; cases y; simp_all [IScalar.val]
+  constructor <;> intro <;>
+  first | simp [*] | apply BitVec.eq_of_toInt_eq; simp [*]
 
-@[simp] theorem Scalar.eq_imp {ty : ScalarTy} (x y : Scalar ty) :
+@[simp] theorem IScalar.eq_imp {ty : IScalarTy} (x y : IScalar ty) :
   (↑x : Int) = ↑y → x = y := (eq_equiv x y).mpr
 
-@[simp] theorem Scalar.lt_equiv {ty : ScalarTy} (x y : Scalar ty) :
-  x < y ↔ (↑x : Int) < ↑y := by simp [LT.lt]
+@[simp] theorem IScalar.lt_equiv {ty : IScalarTy} (x y : IScalar ty) :
+  x < y ↔ (↑x : Int) < ↑y := by
+  rw [LT.lt, instLTIScalar]
 
-@[simp] theorem Scalar.lt_imp {ty : ScalarTy} (x y : Scalar ty) :
+@[simp] theorem IScalar.lt_imp {ty : IScalarTy} (x y : IScalar ty) :
   (↑x : Int) < (↑y) → x < y := (lt_equiv x y).mpr
 
-@[simp] theorem Scalar.le_equiv {ty : ScalarTy} (x y : Scalar ty) :
+@[simp] theorem IScalar.le_equiv {ty : IScalarTy} (x y : IScalar ty) :
   x ≤ y ↔ (↑x : Int) ≤ ↑y := by simp [LE.le]
 
-@[simp] theorem Scalar.le_imp {ty : ScalarTy} (x y : Scalar ty) :
+@[simp] theorem IScalar.le_imp {ty : IScalarTy} (x y : IScalar ty) :
   (↑x : Int) ≤ ↑y → x ≤ y := (le_equiv x y).mpr
 
-instance Scalar.decLt {ty} (a b : Scalar ty) : Decidable (LT.lt a b) := Int.decLt ..
-instance Scalar.decLe {ty} (a b : Scalar ty) : Decidable (LE.le a b) := Int.decLe ..
+instance UScalar.decLt {ty} (a b : UScalar ty) : Decidable (LT.lt a b) := Nat.decLt ..
+instance UScalar.decLe {ty} (a b : UScalar ty) : Decidable (LE.le a b) := Nat.decLe ..
+instance IScalar.decLt {ty} (a b : IScalar ty) : Decidable (LT.lt a b) := Int.decLt ..
+instance IScalar.decLe {ty} (a b : IScalar ty) : Decidable (LE.le a b) := Int.decLe ..
 
-theorem Scalar.eq_of_val_eq {ty} : ∀ {i j : Scalar ty}, Eq i.val j.val → Eq i j
-  | ⟨_, _, _⟩, ⟨_, _, _⟩, rfl => rfl
+theorem UScalar.eq_of_val_eq {ty} : ∀ {i j : UScalar ty}, Eq i.val j.val → Eq i j
+  | ⟨_, _⟩, ⟨_, _⟩, rfl => rfl
 
-theorem Scalar.val_eq_of_eq {ty} {i j : Scalar ty} (h : Eq i j) : Eq i.val j.val :=
-  h ▸ rfl
+theorem IScalar.eq_of_val_eq {ty} : ∀ {i j : IScalar ty}, Eq i.val j.val → Eq i j := by
+  intro i j hEq
+  dcases i; dcases j
+  simp [IScalar.val] at hEq; simp
+  apply BitVec.eq_of_toInt_eq; assumption
 
-theorem Scalar.ne_of_val_ne {ty} {i j : Scalar ty} (h : Not (Eq i.val j.val)) : Not (Eq i j) :=
+theorem UScalar.val_eq_of_eq {ty} {i j : UScalar ty} (h : Eq i j) : Eq i.val j.val := h ▸ rfl
+theorem IScalar.val_eq_of_eq {ty} {i j : IScalar ty} (h : Eq i j) : Eq i.val j.val := h ▸ rfl
+
+theorem UScalar.ne_of_val_ne {ty} {i j : UScalar ty} (h : Not (Eq i.val j.val)) : Not (Eq i j) :=
   fun h' => absurd (val_eq_of_eq h') h
 
-instance (ty : ScalarTy) : DecidableEq (Scalar ty) :=
+theorem IScalar.ne_of_val_ne {ty} {i j : IScalar ty} (h : Not (Eq i.val j.val)) : Not (Eq i j) :=
+  fun h' => absurd (val_eq_of_eq h') h
+
+instance (ty : UScalarTy) : DecidableEq (UScalar ty) :=
   fun i j =>
     match decEq i.val j.val with
-    | isTrue h  => isTrue (Scalar.eq_of_val_eq h)
-    | isFalse h => isFalse (Scalar.ne_of_val_ne h)
+    | isTrue h  => isTrue (UScalar.eq_of_val_eq h)
+    | isFalse h => isFalse (UScalar.ne_of_val_ne h)
 
-@[simp] theorem Scalar.neq_to_neq_val {ty} : ∀ {i j : Scalar ty}, (¬ i = j) ↔ ¬ i.val = j.val := by
+instance (ty : IScalarTy) : DecidableEq (IScalar ty) :=
+  fun i j =>
+    match decEq i.val j.val with
+    | isTrue h  => isTrue (IScalar.eq_of_val_eq h)
+    | isFalse h => isFalse (IScalar.ne_of_val_ne h)
+
+@[simp] theorem UScalar.neq_to_neq_val {ty} : ∀ {i j : UScalar ty}, (¬ i = j) ↔ ¬ i.val = j.val := by
+  simp [eq_equiv]
+
+@[simp] theorem IScalar.neq_to_neq_val {ty} : ∀ {i j : IScalar ty}, (¬ i = j) ↔ ¬ i.val = j.val := by
   simp [eq_equiv]
 
 @[simp]
-theorem Scalar.val_not_eq_imp_not_eq (x y : Scalar ty) (h : ScalarTac.Int.not_eq x.val y.val) :
+theorem UScalar.val_not_eq_imp_not_eq (x y : UScalar ty) (h : ScalarTac.Nat.not_eq x.val y.val) :
   ¬ x = y := by
   simp_all; int_tac
 
-instance (ty: ScalarTy) : Preorder (Scalar ty) where
+@[simp]
+theorem IScalar.val_not_eq_imp_not_eq (x y : IScalar ty) (h : ScalarTac.Int.not_eq x.val y.val) :
+  ¬ x = y := by
+  simp_all; int_tac
+
+instance (ty: UScalarTy) : Preorder (UScalar ty) where
   le_refl := fun a => by simp
   le_trans := fun a b c => by
     intro Hab Hbc
-    exact (le_trans ((Scalar.le_equiv _ _).1 Hab) ((Scalar.le_equiv _ _).1 Hbc))
+    exact (le_trans ((UScalar.le_equiv _ _).1 Hab) ((UScalar.le_equiv _ _).1 Hbc))
   lt_iff_le_not_le := fun a b => by
-    trans (a: Int) < (b: Int); exact (Scalar.lt_equiv _ _)
+    trans (a: Nat) < (b: Nat); exact (UScalar.lt_equiv _ _)
+    trans (a: Nat) ≤ (b: Nat) ∧ ¬ (b: Nat) ≤ (a: Nat); exact lt_iff_le_not_le
+    repeat rewrite [← UScalar.le_equiv]; rfl
+
+instance (ty: IScalarTy) : Preorder (IScalar ty) where
+  le_refl := fun a => by simp
+  le_trans := fun a b c => by
+    intro Hab Hbc
+    exact (le_trans ((IScalar.le_equiv _ _).1 Hab) ((IScalar.le_equiv _ _).1 Hbc))
+  lt_iff_le_not_le := fun a b => by
+    trans (a: Int) < (b: Int); exact (IScalar.lt_equiv _ _)
     trans (a: Int) ≤ (b: Int) ∧ ¬ (b: Int) ≤ (a: Int); exact lt_iff_le_not_le
-    repeat rewrite [← Scalar.le_equiv]; rfl
+    repeat rewrite [← IScalar.le_equiv]; rfl
 
-instance (ty: ScalarTy) : PartialOrder (Scalar ty) where
-  le_antisymm := fun a b Hab Hba => Scalar.eq_imp _ _ ((@le_antisymm Int _ _ _ ((Scalar.le_equiv a b).1 Hab) ((Scalar.le_equiv b a).1 Hba)))
+instance (ty: UScalarTy) : PartialOrder (UScalar ty) where
+  le_antisymm := fun a b Hab Hba =>
+    UScalar.eq_imp _ _ ((@le_antisymm Nat _ _ _ ((UScalar.le_equiv a b).1 Hab) ((UScalar.le_equiv b a).1 Hba)))
 
-instance ScalarDecidableLE (ty: ScalarTy) : DecidableRel (· ≤ · : Scalar ty -> Scalar ty -> Prop) := by
-  simp [instLEScalar]
+instance (ty: IScalarTy) : PartialOrder (IScalar ty) where
+  le_antisymm := fun a b Hab Hba =>
+    IScalar.eq_imp _ _ ((@le_antisymm Int _ _ _ ((IScalar.le_equiv a b).1 Hab) ((IScalar.le_equiv b a).1 Hba)))
+
+instance UScalarDecidableLE (ty: UScalarTy) : DecidableRel (· ≤ · : UScalar ty -> UScalar ty -> Prop) := by
+  simp [instLEUScalar]
   -- Lift this to the decidability of the Int version.
   infer_instance
 
-instance (ty: ScalarTy) : LinearOrder (Scalar ty) where
+instance IScalarDecidableLE (ty: IScalarTy) : DecidableRel (· ≤ · : IScalar ty -> IScalar ty -> Prop) := by
+  simp [instLEIScalar]
+  -- Lift this to the decidability of the Int version.
+  infer_instance
+
+instance (ty: UScalarTy) : LinearOrder (UScalar ty) where
+  le_total := fun a b => by
+    rcases (Nat.le_total a b) with H | H
+    left; exact (UScalar.le_equiv _ _).2 H
+    right; exact (UScalar.le_equiv _ _).2 H
+  decidableLE := UScalarDecidableLE ty
+
+instance (ty: IScalarTy) : LinearOrder (IScalar ty) where
   le_total := fun a b => by
     rcases (Int.le_total a b) with H | H
-    left; exact (Scalar.le_equiv _ _).2 H
-    right; exact (Scalar.le_equiv _ _).2 H
-  decidableLE := ScalarDecidableLE ty
+    left; exact (IScalar.le_equiv _ _).2 H
+    right; exact (IScalar.le_equiv _ _).2 H
+  decidableLE := IScalarDecidableLE ty
 
--- Coercion theorems
--- This is helpful whenever you want to "push" casts to the innermost nodes
--- and make the cast normalization happen more magically.
+/-! Coercion theorems
+
+    This is helpful whenever you want to "push" casts to the innermost nodes
+    and make the cast normalization happen more magically. -/
 
 @[simp, norm_cast]
-theorem coe_max {ty: ScalarTy} (a b: Scalar ty): ↑(Max.max a b) = (Max.max (↑a) (↑b): ℤ) := by
+theorem UScalar.coe_max {ty: UScalarTy} (a b: UScalar ty): ↑(Max.max a b) = (Max.max (↑a) (↑b): ℕ) := by
   -- TODO: there should be a shorter way to prove this.
   rw [max_def, max_def]
   split_ifs <;> simp_all
 
--- Max theory
+@[simp, norm_cast]
+theorem IScalar.coe_max {ty: IScalarTy} (a b: IScalar ty): ↑(Max.max a b) = (Max.max (↑a) (↑b): ℤ) := by
+  -- TODO: there should be a shorter way to prove this.
+  rw [max_def, max_def]
+  split_ifs <;> simp_all
+
+/-! Max theory -/
 -- TODO: do the min theory later on.
 
-theorem Scalar.zero_le_unsigned {ty} (s: ¬ ty.isSigned) (x: Scalar ty): Scalar.ofInt 0 (by simp) ≤ x := by
-  apply (Scalar.le_equiv _ _).2
-  convert x.hmin
-  cases ty <;> simp [ScalarTy.isSigned] at s <;> simp [Scalar.min]
+theorem UScalar.zero_le {ty} (x: UScalar ty): UScalar.ofNat 0 (by simp) ≤ x := by simp
 
 @[simp]
-theorem Scalar.max_unsigned_left_zero_eq {ty} [s: Fact (¬ ty.isSigned)] (x: Scalar ty):
-  Max.max (Scalar.ofInt 0 (by simp)) x = x := max_eq_right (Scalar.zero_le_unsigned s.out x)
+theorem UScalar.max_left_zero_eq {ty} (x: UScalar ty):
+  Max.max (UScalar.ofNat 0 (by simp)) x = x := max_eq_right (UScalar.zero_le x)
 
 @[simp]
-theorem Scalar.max_unsigned_right_zero_eq {ty} [s: Fact (¬ ty.isSigned)] (x: Scalar ty):
-  Max.max x (Scalar.ofInt 0 (by simp)) = x := max_eq_left (Scalar.zero_le_unsigned s.out x)
+theorem UScalar.max_right_zero_eq {ty} (x: UScalar ty):
+  Max.max x (UScalar.ofNat 0 (by simp)) = x := max_eq_left (UScalar.zero_le x)
 
--- Some conversions
-@[simp] abbrev Scalar.toNat {ty} (x : Scalar ty) : Nat := x.val.toNat
-@[simp] abbrev U8.toNat    (x : U8) : Nat := x.val.toNat
-@[simp] abbrev U16.toNat   (x : U16) : Nat := x.val.toNat
-@[simp] abbrev U32.toNat   (x : U32) : Nat := x.val.toNat
-@[simp] abbrev U64.toNat   (x : U64) : Nat := x.val.toNat
-@[simp] abbrev U128.toNat  (x : U128) : Nat := x.val.toNat
-@[simp] abbrev Usize.toNat (x : Usize) : Nat := x.val.toNat
+/-! Some conversions -/
 @[simp] abbrev I8.toNat    (x : I8) : Nat := x.val.toNat
 @[simp] abbrev I16.toNat   (x : I16) : Nat := x.val.toNat
 @[simp] abbrev I32.toNat   (x : I32) : Nat := x.val.toNat
@@ -633,38 +769,41 @@ theorem Scalar.max_unsigned_right_zero_eq {ty} [s: Fact (¬ ty.isSigned)] (x: Sc
 @[simp] abbrev I128.toNat  (x : I128) : Nat := x.val.toNat
 @[simp] abbrev Isize.toNat (x : Isize) : Nat := x.val.toNat
 
-@[simp]
-theorem Scalar.unsigned_ofNat_toNat (x : Scalar ty) (h : ¬ ty.isSigned := by decide) :
-  (x.toNat : Int) = x.val := by
-  have := x.hmin
-  simp; cases ty <;> simp_all [min]
+def U8.bv (x : U8)   : BitVec 8 := UScalar.bv x
+def U16.bv (x : U16) : BitVec 16 := UScalar.bv x
+def U32.bv (x : U32) : BitVec 32 := UScalar.bv x
+def U64.bv (x : U64) : BitVec 64 := UScalar.bv x
+def U128.bv (x : U128) : BitVec 128 := UScalar.bv x
+def Usize.bv (x : Usize) : BitVec size_num_bits := UScalar.bv x
 
-@[scalar_tac x.toNat] theorem U8.unsigned_ofNat_toNat (x : U8) : (x.toNat : Int) = x.val := Scalar.unsigned_ofNat_toNat x
-@[scalar_tac x.toNat] theorem U16.unsigned_ofNat_toNat (x : U16) : (x.toNat : Int) = x.val := Scalar.unsigned_ofNat_toNat x
-@[scalar_tac x.toNat] theorem U32.unsigned_ofNat_toNat (x : U32) : (x.toNat : Int) = x.val := Scalar.unsigned_ofNat_toNat x
-@[scalar_tac x.toNat] theorem U64.unsigned_ofNat_toNat (x : U64) : (x.toNat : Int) = x.val := Scalar.unsigned_ofNat_toNat x
-@[scalar_tac x.toNat] theorem U128.unsigned_ofNat_toNat (x : U128) : (x.toNat : Int) = x.val := Scalar.unsigned_ofNat_toNat x
-@[scalar_tac x.toNat] theorem Usize.unsigned_ofNat_toNat (x : Usize) : (x.toNat : Int) = x.val := Scalar.unsigned_ofNat_toNat x
+def I8.bv (x : I8) : BitVec 8 := IScalar.bv x
+def I16.bv (x : I16) : BitVec 16 := IScalar.bv x
+def I32.bv (x : I32) : BitVec 32 := IScalar.bv x
+def I64.bv (x : I64) : BitVec 64 := IScalar.bv x
+def I128.bv (x : I128) : BitVec 128 := IScalar.bv x
+def Isize.bv (x : Isize) : BitVec size_num_bits := IScalar.bv x
 
-@[simp]
-theorem Scalar.unsigned_add_nat_toNat (h : ¬ ty.isSigned) (x : Scalar ty) (n : Nat) :
-  (x.val + n).toNat = x.val.toNat + n := by
-  cases ty <;> simp_all <;> int_tac
+@[simp] theorem UScalar.bv_toNat_eq {ty : UScalarTy} (x : UScalar ty) :
+  (UScalar.bv x).toNat  = x.val := by
+  simp [val]
 
-@[simp]
-theorem Scalar.unsigned_nat_add_toNat (h : ¬ ty.isSigned) (x : Scalar ty) (n : Nat) :
-  (n + x.val).toNat = x.val.toNat + n := by
-  cases ty <;> simp_all <;> int_tac
+@[simp] theorem U8.bv_toNat_eq (x : U8) : x.bv.toNat = x.val := by apply UScalar.bv_toNat_eq
+@[simp] theorem U16.bv_toNat_eq (x : U16) : x.bv.toNat = x.val := by apply UScalar.bv_toNat_eq
+@[simp] theorem U32.bv_toNat_eq (x : U32) : x.bv.toNat = x.val := by apply UScalar.bv_toNat_eq
+@[simp] theorem U64.bv_toNat_eq (x : U64) : x.bv.toNat = x.val := by apply UScalar.bv_toNat_eq
+@[simp] theorem U128.bv_toNat_eq (x : U128) : x.bv.toNat = x.val := by apply UScalar.bv_toNat_eq
+@[simp] theorem Usize.bv_toNat_eq (x : Usize) : x.bv.toNat = x.val := by apply UScalar.bv_toNat_eq
 
-@[simp]
-theorem Scalar.unsigned_add_pos_toNat (h : ¬ ty.isSigned) (x : Scalar ty) (n : Int) (h' : 0 ≤ n) :
-  (x.val + n).toNat = x.val.toNat + n.toNat := by
-  cases ty <;> simp_all <;> int_tac
+@[simp] theorem IScalar.bv_toInt_eq {ty : IScalarTy} (x : IScalar ty) :
+  (IScalar.bv x).toInt  = x.val := by
+  simp [val]
 
-@[simp]
-theorem Scalar.unsigned_pos_add_toNat (h : ¬ ty.isSigned) (x : Scalar ty) (n : Int) (h' : 0 ≤ n) :
-  (n + x.val).toNat = n.toNat + x.val.toNat := by
-  cases ty <;> simp_all <;> int_tac
+@[simp] theorem I8.bv_toInt_eq (x : I8) : x.bv.toInt = x.val := by apply IScalar.bv_toInt_eq
+@[simp] theorem I16.bv_toInt_eq (x : I16) : x.bv.toInt = x.val := by apply IScalar.bv_toInt_eq
+@[simp] theorem I32.bv_toInt_eq (x : I32) : x.bv.toInt = x.val := by apply IScalar.bv_toInt_eq
+@[simp] theorem I64.bv_toInt_eq (x : I64) : x.bv.toInt = x.val := by apply IScalar.bv_toInt_eq
+@[simp] theorem I128.bv_toInt_eq (x : I128) : x.bv.toInt = x.val := by apply IScalar.bv_toInt_eq
+@[simp] theorem Isize.bv_toInt_eq (x : Isize) : x.bv.toInt = x.val := by apply IScalar.bv_toInt_eq
 
 end Std
 
